instead of moving GenSep to use nat, allow both nat and addr
unfortunately, this means duplicating GenSep: there's now
GenSep.v (for addr-based memories) and GenSepN.v (for nat-based memories)

src/GenSep.v
@@ -26,26 +26,37 @@ Set Implicit Arguments.
  * object that maps inode numbers (list positions) into files (or None, if the
  * inode number is too big).  For now, this always uses [addr] as the index.
  *)
-Definition list2mem (A: Type) (l: list A) : (@mem nat eq_nat_dec A) :=
-  fun a => selN (map (@Some A) l) a None.
+Definition list2mem (A: Type) (l: list A) : @mem addr (@weq addrlen) A :=
+  fun a => sel (map (@Some A) l) a None.
+
+Theorem list2mem_ptsto_bounds: forall A F (l: list A) i x,
+  (F * i |-> x)%pred (list2mem l) -> wordToNat i < length l.
+Proof.
+  intros.
+  unfold list2mem in H.
+  apply ptsto_valid' in H.
+  destruct (lt_dec (wordToNat i) (length l)); auto.
+  unfold sel in H. rewrite nth_selN_eq in H.
+  rewrite nth_overflow in H by (rewrite map_length; omega); discriminate.
+Qed.
 
 
 Theorem list2mem_oob : forall A (l : list A) i,
-  i >= length l
+  wordToNat i >= length l
   -> (list2mem l) i = None.
 Proof.
   unfold list2mem; intros.
-  rewrite selN_oob; auto.
+  unfold sel; rewrite selN_oob; auto.
   rewrite map_length; auto.
 Qed.
 
 
 Theorem list2mem_inbound: forall A F (l : list A) i x,
   (F * i |-> x)%pred (list2mem l)
-  -> i < length l.
+  -> wordToNat i < length l.
 Proof.
   intros.
-  destruct (lt_dec i (length l)); auto; exfalso.
+  destruct (lt_dec (wordToNat i) (length l)); auto; exfalso.
   apply not_lt in n.
   apply list2mem_oob in n.
   apply ptsto_valid' in H.
@@ -56,36 +67,37 @@ Qed.
 
 Theorem list2mem_sel: forall A F (l: list A) i x def,
   (F * i |-> x)%pred (list2mem l)
-  -> x = selN l i def.
+  -> x = sel l i def.
 Proof.
   intros.
-  assert (i < length l).
+  assert (wordToNat i < length l).
   eapply list2mem_inbound; eauto.
   unfold list2mem in H.
   apply ptsto_valid' in H.
-  erewrite selN_map in H by auto.
+  erewrite sel_map in H by auto.
   inversion H; eauto.
 Qed.
 
 
 Lemma listupd_progupd: forall A l i (v : A),
-  i < length l
-  -> list2mem (updN l i v) = Prog.upd (list2mem l) i v.
+  wordToNat i < length l
+  -> list2mem (upd l i v) = Prog.upd (list2mem l) i v.
 Proof.
   intros.
   apply functional_extensionality; intro.
-  unfold list2mem, Prog.upd.
+  unfold list2mem, sel, upd, Prog.upd.
   autorewrite with core.
 
-  destruct (eq_nat_dec x i).
+  destruct (weq x i).
   subst; erewrite selN_updN_eq; auto.
   rewrite map_length; auto.
   erewrite selN_updN_ne; auto.
+  word2nat_simpl; omega.
 Qed.
 
 Theorem list2mem_upd: forall A F (l: list A) i x y,
   (F * i |-> x)%pred (list2mem l)
-  -> (F * i |-> y)%pred (list2mem (updN l i y)).
+  -> (F * i |-> y)%pred (list2mem (upd l i y)).
 Proof.
   intros.
   rewrite listupd_progupd; auto.
@@ -96,33 +108,46 @@ Proof.
 Qed.
 
 
-Theorem listapp_progupd: forall A l (a : A),
-  list2mem (l ++ a :: nil) = Prog.upd (list2mem l) (length l) a.
+Theorem listapp_progupd: forall A l (a : A) (b : addr),
+  length l <= wordToNat b
+  -> list2mem (l ++ a :: nil) = Prog.upd (list2mem l) $ (length l) a.
 Proof.
   intros.
   apply functional_extensionality; intro.
-  unfold list2mem, Prog.upd.
+  unfold list2mem, sel, upd, Prog.upd.
 
-  destruct (lt_dec x (length l)).
-  - subst; rewrite selN_map with (default' := a).
-    destruct (eq_nat_dec x (length l)); subst.
-    + rewrite selN_last; auto.
+  destruct (wlt_dec x $ (length l)).
+  - apply wlt_lt in w.
+    erewrite wordToNat_natToWord_bound in w; eauto.
+    subst; rewrite selN_map with (default' := a).
+    destruct (weq x $ (length l)); subst.
+    + erewrite wordToNat_natToWord_bound in *; eauto.
+      rewrite selN_last; auto.
     + rewrite selN_map with (default' := a); auto.
       rewrite selN_app; auto.
     + rewrite app_length; simpl; omega.
-  - destruct (eq_nat_dec x (length l)).
+  - destruct (weq x $ (length l)).
     + subst; erewrite selN_map with (default' := a).
       rewrite selN_last; auto.
+      eapply wordToNat_natToWord_bound; eauto.
+      erewrite wordToNat_natToWord_bound; eauto.
       rewrite app_length; simpl; omega.
-    + repeat erewrite selN_oob with (def := None); try rewrite map_length; auto.
-      omega.
+    + apply wle_le in n.
+      erewrite wordToNat_natToWord_bound in n; eauto.
+      repeat erewrite selN_oob with (def := None); try rewrite map_length; auto.
       rewrite app_length; simpl; intuition.
+      rewrite Nat.add_1_r; apply lt_le_S.
+      apply le_lt_or_eq in n; intuition.
+      contradict n0; rewrite H0.
+      apply wordToNat_inj.
+      erewrite wordToNat_natToWord_bound; eauto.
 Qed.
 
 
-Theorem list2mem_app: forall A (F : @pred _ _ A) l a,
-  F (list2mem l)
-  -> (F * (length l) |-> a)%pred (list2mem (l ++ a :: nil)).
+Theorem list2mem_app: forall A (F : @pred addr (@weq addrlen) A) l a (b : addr),
+  length l <= wordToNat b
+  -> F (list2mem l)
+  -> (F * $ (length l) |-> a)%pred (list2mem (l ++ a :: nil)).
 Proof.
   intros.
   erewrite listapp_progupd; eauto.
@@ -130,92 +155,92 @@ Proof.
   unfold list2mem, sel.
   rewrite selN_oob; auto.
   rewrite map_length.
-  omega.
+  erewrite wordToNat_natToWord_bound; eauto.
 Qed.
 
 
-Theorem list2mem_removelast_is : forall A l (def : A),
-  l <> nil
+Theorem list2mem_removelast_is : forall A l (def : A) (b : addr),
+  l <> nil -> length l <= wordToNat b
   -> list2mem (removelast l) =
-     fun i => if (lt_dec i (length l - 1)) then Some (selN l i def) else None.
+     fun i => if (wlt_dec i $ (length l - 1)) then Some (sel l i def) else None.
 Proof.
   intros; apply functional_extensionality; intros.
-  destruct (lt_dec x (length l - 1)); unfold list2mem, sel.
-  - rewrite selN_map with (default' := def).
+  destruct (wlt_dec x $ (length l - 1)); unfold list2mem, sel.
+  - assert (wordToNat x < length l - 1); apply wlt_lt in w.
+    erewrite wordToNat_natToWord_bound with (bound:=b) in w by omega; auto.
+    rewrite selN_map with (default' := def).
     rewrite selN_removelast by omega; auto.
     rewrite length_removelast by auto; omega.
   - rewrite selN_oob; auto.
     rewrite map_length.
     rewrite length_removelast by auto.
-    omega.
+    apply wle_le in n.
+    rewrite wordToNat_natToWord_bound with (bound:=b) in n by omega; auto.
 Qed.
 
 
-Theorem list2mem_removelast_list2mem : forall A (l : list A) (def : A),
-  l <> nil
+Theorem list2mem_removelast_list2mem : forall A (l : list A) (b : addr),
+  l <> nil -> length l <= wordToNat b
   -> list2mem (removelast l) =
-     fun i => if (eq_nat_dec i (length l - 1)) then None else (list2mem l) i.
+     fun i => if (weq i $ (length l - 1)) then None else (list2mem l) i.
 Proof.
   intros; apply functional_extensionality; intros.
+  assert (exists def, firstn 1 l = def :: nil) as Hdef.
+  destruct l; try congruence.
+  exists a; eauto.
+  destruct Hdef as [def _].
+
   erewrite list2mem_removelast_is with (def := def) by eauto.
-  unfold list2mem.
-  destruct (lt_dec x (length l - 1));
-  destruct (eq_nat_dec x (length l - 1)); subst; intuition.
-  omega.
+  unfold list2mem, sel.
+  destruct (wlt_dec x $ (length l - 1));
+  destruct (weq x $ (length l - 1)); subst; intuition.
+  apply wlt_lt in w; omega.
   erewrite selN_map with (default' := def); auto.
-  omega.
+  apply wlt_lt in w; rewrite wordToNat_natToWord_bound with (bound:=b) in w by omega; omega.
   erewrite selN_oob; auto.
   rewrite map_length.
-  omega.
+  assert ($ (length l - 1) < x)%word.
+  destruct (weq $ (length l - 1) x); intuition.
+  apply wlt_lt in H1; rewrite wordToNat_natToWord_bound with (bound:=b) in H1 by omega; omega.
 Qed.
 
 
-Lemma mem_disjoint_either: forall AT AEQ V (m1 m2 : @mem AT AEQ V) a v,
-  mem_disjoint m1 m2
-  -> m1 a = Some v -> m2 a = None.
-Proof.
-  unfold mem_disjoint; intros; firstorder.
-  pose proof (H a); firstorder.
-  pose proof (H1 v); firstorder.
-  destruct (m2 a); auto.
-  pose proof (H2 v0); firstorder.
-Qed.
-
-
-Theorem list2mem_removelast: forall A F (l : list A) v,
-  l <> nil
-  -> (F * (length l - 1) |-> v)%pred (list2mem l)
+Theorem list2mem_removelast: forall A F (l : list A) v (b : addr),
+  l <> nil -> length l <= wordToNat b
+  -> (F * $ (length l - 1) |-> v)%pred (list2mem l)
   -> F (list2mem (removelast l)).
 Proof.
   unfold_sep_star; unfold ptsto; intuition; repeat deex.
   assert (x = list2mem (removelast l)); subst; auto.
   apply functional_extensionality; intros.
-  rewrite list2mem_removelast_list2mem; auto.
+  rewrite list2mem_removelast_list2mem with (b:=b); auto.
 
-  destruct (eq_nat_dec x1 (length l - 1)); subst.
-  apply mem_disjoint_comm in H0. 
+  destruct (weq x1 $ (length l - 1)); subst.
+  apply mem_disjoint_comm in H1. 
   eapply mem_disjoint_either; eauto.
 
-  rewrite H1; unfold mem_union.
+  rewrite H2; unfold mem_union.
   destruct (x x1); subst; simpl; auto.
-  apply eq_sym; apply H5; auto.
+  apply eq_sym; apply H6; auto.
 Qed.
 
 
-Theorem list2mem_array: forall  A (l : list A),
-  arrayN 0 l (list2mem l).
+Theorem list2mem_array: forall  A (l : list A) (b : addr),
+  length l <= wordToNat b
+  -> array $0 l $1 (list2mem l).
 Proof.
   induction l using rev_ind; intros; firstorder; simpl.
-  erewrite listapp_progupd; try omega.
-  eapply arrayN_app_progupd; try omega.
-  eauto.
+  rewrite app_length in H; simpl in H.
+  erewrite listapp_progupd with (b := b); try omega.
+  eapply array_app_progupd with (b := b); try omega.
+  apply IHl with (b := b); omega.
 Qed.
 
 
 (* Alternative variants of [list2mem] that are more induction-friendly *)
-Definition list2mem_off (A: Type) (start : nat) (l: list A) : (nat -> option A) :=
-  fun a => if lt_dec a start then None
-                             else selN (map (@Some A) l) (a - start) None.
+Definition list2mem_off (A: Type) (start : nat) (l: list A) : (addr -> option A) :=
+  fun a => if lt_dec (wordToNat a) start then None
+                                         else selN (map (@Some A) l) (wordToNat a - start) None.
 
 Theorem list2mem_off_eq : forall A (l : list A), list2mem l = list2mem_off 0 l.
 Proof.
@@ -225,114 +250,130 @@ Proof.
   reflexivity.
 Qed.
 
-Fixpoint list2mem_fix (A : Type) (start : nat) (l : list A) : (nat -> option A) :=
+Fixpoint list2mem_fix (A : Type) (start : nat) (l : list A) : (addr -> option A) :=
   match l with
   | nil => fun a => None
-  | h :: l' => fun a => if eq_nat_dec a start then Some h else list2mem_fix (S start) l' a
+  | h :: l' => fun a => if eq_nat_dec (wordToNat a) start then Some h else list2mem_fix (S start) l' a
   end.
 
 Lemma list2mem_fix_below : forall (A : Type) (l : list A) start a,
-  a < start -> list2mem_fix start l a = None.
+  wordToNat a < start -> list2mem_fix start l a = None.
 Proof.
   induction l; auto; simpl; intros.
-  destruct (eq_nat_dec a0 start); [omega |].
+  destruct (eq_nat_dec (wordToNat a0) start); [omega |].
   apply IHl; omega.
 Qed.
 
-Theorem list2mem_fix_off_eq : forall A (l : list A) n,
-  list2mem_off n l = list2mem_fix n l.
+Theorem list2mem_fix_off_eq : forall A (l : list A) n (b : addr),
+  length l + n <= wordToNat b -> list2mem_off n l = list2mem_fix n l.
 Proof.
   induction l; intros; apply functional_extensionality; intros.
-  unfold list2mem_off; destruct (lt_dec x n); auto.
+  unfold list2mem_off; destruct (lt_dec (wordToNat x) n); auto.
 
   unfold list2mem_off; simpl in *.
 
-  destruct (lt_dec x n).
-  destruct (eq_nat_dec x n); [omega |].
+  destruct (lt_dec (wordToNat x) n).
+  destruct (eq_nat_dec (wordToNat x) n); [omega |].
   rewrite list2mem_fix_below by omega.
   auto.
 
-  destruct (eq_nat_dec x n).
+  destruct (eq_nat_dec (wordToNat x) n).
   rewrite e; replace (n-n) with (0) by omega; auto.
 
-  assert (x - n <> 0) by omega.
-  destruct (x - n) eqn:Hxn; try congruence.
+  assert (wordToNat x - n <> 0) by omega.
+  destruct (wordToNat x - n) eqn:Hxn; try congruence.
 
-  rewrite <- IHl.
+  rewrite <- IHl with (b:=b) by omega.
   unfold list2mem_off.
 
-  destruct (lt_dec x (S n)); [omega |].
+  destruct (lt_dec (wordToNat x) (S n)); [omega |].
   f_equal; omega.
 Qed.
 
-Theorem list2mem_fix_eq : forall A (l : list A),
-  list2mem l = list2mem_fix 0 l.
+Theorem list2mem_fix_eq : forall A (l : list A) (b : addr),
+  length l <= wordToNat b -> list2mem l = list2mem_fix 0 l.
 Proof.
   intros.
   rewrite list2mem_off_eq.
   eapply list2mem_fix_off_eq.
+  rewrite <- plus_n_O.
+  eassumption.
 Qed.
 
 
 Lemma list2mem_nil_array : forall A (l : list A) start,
-  arrayN start l (list2mem nil) -> l = nil.
+  array $ start l $1 (list2mem nil) -> l = nil.
 Proof.
   destruct l; simpl; auto.
   unfold_sep_star; unfold ptsto, list2mem, sel; simpl; intros.
   repeat deex.
   unfold mem_union in H0.
-  apply equal_f with (start) in H0.
+  apply equal_f with ($ start) in H0.
   rewrite H2 in H0.
   congruence.
 Qed.
 
-Lemma list2mem_array_nil : forall A (l : list A) start,
-  arrayN start nil (list2mem_fix start l) -> l = nil.
+Lemma list2mem_array_nil : forall A (l : list A) start (b : addr),
+  start <= wordToNat b -> array $ start nil $1 (list2mem_fix start l) -> l = nil.
 Proof.
   destruct l; simpl; auto.
   unfold list2mem, sel, emp; intros.
-  pose proof (H start).
+  pose proof (H0 $ start).
+  erewrite wordToNat_natToWord_bound in H1 by eauto.
   destruct (eq_nat_dec start start); simpl in *; congruence.
 Qed.
 
-Theorem list2mem_array_eq': forall A (l' l : list A) start,
-  arrayN start l (list2mem_fix start l')
+Theorem list2mem_array_eq': forall A (l' l : list A) (b : addr) start,
+  array $ start l $1 (list2mem_fix start l')
+  -> length l + start <= wordToNat b
+  -> length l' + start <= wordToNat b
   -> l' = l.
 Proof.
   induction l'; simpl; intros.
   - erewrite list2mem_nil_array; eauto.
   - destruct l.
-    + eapply list2mem_array_nil with (start:=start).
+    + eapply list2mem_array_nil with (start:=start) (b:=b).
+      omega.
       auto.
     + simpl in *.
       unfold sep_star in H; rewrite sep_star_is in H; unfold sep_star_impl in H.
       repeat deex.
-      unfold ptsto in H1; destruct H1.
+      unfold ptsto in H3; destruct H3.
       f_equal.
-      * eapply equal_f with (start) in H0 as H0'.
-        unfold mem_union in H0'.
-        rewrite H1 in H0'.
+      * eapply equal_f with ($ start) in H2 as H2'.
+        erewrite wordToNat_natToWord_bound with (bound:=b) in H2' by omega.
+
+        unfold mem_union in H2'.
+        rewrite H3 in H2'.
         destruct (eq_nat_dec start start); congruence.
-      * apply IHl' with (start:=S start); eauto; try omega.
+      * apply IHl' with (b:=b) (start:=S start); eauto; try omega.
+        replace ($ start ^+ $1) with (natToWord addrlen (S start)) in H5 by words.
         assert (x0 = list2mem_fix (S start) l'); subst; auto.
 
         apply functional_extensionality; intros.
-        unfold mem_union in H0.
-        apply equal_f with x1 in H0.
-        destruct (eq_nat_dec x1 start).
+        unfold mem_union in H2.
+        apply equal_f with x1 in H2.
+        destruct (eq_nat_dec (wordToNat x1) start).
 
         rewrite list2mem_fix_below by omega.
         eapply mem_disjoint_either.
         eauto.
-        rewrite <- e in H1.
+        rewrite <- e in H3.
+        rewrite natToWord_wordToNat in *.
         eauto.
 
-        rewrite H0.
-        rewrite H2; auto.
+        rewrite H2.
+        rewrite H4; auto.
+        intro; apply n.
+        rewrite <- H6.
+        rewrite wordToNat_natToWord_bound with (bound:=b); auto.
+        omega.
 Qed.
 
-Theorem list2mem_array_eq: forall A (l' l : list A),
-  arrayN 0 l (list2mem l')
+Theorem list2mem_array_eq: forall A (l' l : list A) (b : addr),
+  array $0 l $1 (list2mem l')
+  -> length l <= wordToNat b
+  -> length l' <= wordToNat b
   -> l' = l.
 Proof.
   intros; eapply list2mem_array_eq' with (start:=0); try rewrite <- plus_n_O; eauto.
@@ -340,100 +381,122 @@ Proof.
 Qed.
 
 
-Theorem list2mem_array_app_eq: forall A V (F : @pred _ eq_nat_dec V) (l l' : list A) a,
-  (arrayN 0 l * (length l) |-> a)%pred (list2mem l')
+Theorem list2mem_array_app_eq: forall A V (F : @pred addr (@weq addrlen) V) (l l' : list A) a (b : addr),
+  length l < wordToNat b
+  -> length l' <= wordToNat b
+  -> (array $0 l $1 * $ (length l) |-> a)%pred (list2mem l')
   -> l' = (l ++ a :: nil).
 Proof.
   intros.
-  rewrite list2mem_array_eq with (l':=l') (l:=l++a::nil); eauto.
+  rewrite list2mem_array_eq with (l':=l') (l:=l++a::nil) (b:=b); eauto;
+    [ | rewrite app_length; simpl; omega ].
   pred_apply.
-  rewrite <- isolateN_bwd with (vs:=l++a::nil) (i:=length l) by
-    ( rewrite app_length; simpl; omega ).
+  rewrite <- isolate_bwd with (vs:=l++a::nil) (i:=$ (length l)) by
+    ( rewrite wordToNat_natToWord_bound with (bound:=b) by omega;
+      rewrite app_length; simpl; omega ).
+  unfold sel.
+  erewrite wordToNat_natToWord_bound with (bound:=b) by omega.
   rewrite firstn_app by auto.
   replace (S (length l)) with (length (l ++ a :: nil)) by (rewrite app_length; simpl; omega).
   rewrite skipn_oob by omega; simpl.
-  instantiate (1:=a).
+  instantiate (y:=a).
   rewrite selN_last by auto.
   cancel.
 Qed.
 
 
-Definition arrayN_ex A (vs : list A) i :=
-  (arrayN 0 (firstn i vs) * arrayN (i + 1) (skipn (S i) vs))%pred.
+Definition array_ex A (vs : list A) i :=
+  ( array $0 (firstn (wordToNat i) vs) $1 *
+    array (i ^+ $1) (skipn (S (wordToNat i)) vs) $1)%pred.
 
 
-Theorem arrayN_except : forall V vs (def : V) i,
-  i < length vs
-  -> arrayN 0 vs <=p=> (arrayN_ex vs i) * (i |-> selN vs i def).
+Theorem array_except : forall V vs (def : V) (i : addr),
+  wordToNat i < length vs
+  -> array $0 vs $1 <=p=> (array_ex vs i) * (i |-> sel vs i def).
 Proof.
-  intros; unfold arrayN_ex.
-  erewrite arrayN_isolate with (default := def); eauto.
-  simpl.
+  intros; unfold array_ex.
+  erewrite array_isolate with (default := def); eauto.
+  ring_simplify ($ (0) ^+ i ^* $ (1)).
+  ring_simplify ($ (0) ^+ (i ^+ $ (1)) ^* $ (1)).
   unfold piff; split; cancel.
 Qed.
 
 
-Theorem arrayN_except_upd : forall V vs (v : V) i,
-  i < length vs
-  -> arrayN 0 (updN vs i v) <=p=> (arrayN_ex vs i) * (i |-> v).
+Theorem array_except_upd : forall V vs (v : V) (i : addr),
+  wordToNat i < length vs
+  -> array $0 (upd vs i v) $1 <=p=> (array_ex vs i) * (i |-> v).
 Proof.
-  intros; unfold arrayN_ex.
-  erewrite arrayN_isolate_upd; eauto.
-  simpl.
+  intros; unfold array_ex.
+  erewrite array_isolate_upd; eauto.
+  ring_simplify ($ (0) ^+ i ^* $ (1)).
+  ring_simplify ($ (0) ^+ (i ^+ $ (1)) ^* $ (1)).
   unfold piff; split; cancel.
 Qed.
 
 
-Theorem list2mem_array_pick : forall V l (def : V) i,
-  i < length l
-  -> (arrayN_ex l i * i |-> selN l i def)%pred (list2mem l).
+Theorem list2mem_array_pick : forall V l (def : V) (i b : addr),
+  length l <= wordToNat b
+  -> wordToNat i < length l
+  -> (array_ex l i * i |-> sel l i def)%pred (list2mem l).
 Proof.
   intros.
-  eapply arrayN_except; eauto.
+  eapply array_except; eauto.
   eapply list2mem_array; eauto.
 Qed.
 
-Theorem list2mem_array_upd : forall V ol nl (v : V) i,
-  (arrayN_ex ol i * i |-> v)%pred (list2mem nl)
-  -> i < length ol
-  -> nl = updN ol i v.
+Theorem list2mem_array_upd : forall V ol nl (v : V) (i b : addr),
+  (array_ex ol i * i |-> v)%pred (list2mem nl)
+  -> length ol <= wordToNat b
+  -> length nl <= wordToNat b
+  -> wordToNat i < length ol
+  -> nl = upd ol i v.
 Proof.
   intros.
-  eapply list2mem_array_eq; autorewrite with core; auto.
+  eapply list2mem_array_eq with (b := b); autorewrite with core; auto.
   pred_apply.
-  rewrite arrayN_except_upd; auto.
+  rewrite array_except_upd; auto.
 Qed.
 
-Theorem list2mem_array_updN : forall V ol nl (v : V) i,
-  (arrayN_ex ol i * i |-> v)%pred (list2mem nl)
-  -> i < length ol
-  -> updN ol i v = nl.
+Theorem list2mem_array_updN : forall V ol nl (v : V) (i b : addr),
+  (array_ex ol i * i |-> v)%pred (list2mem nl)
+  -> length ol <= wordToNat b
+  -> length nl <= wordToNat b
+  -> wordToNat i < length ol
+  -> updN ol (wordToNat i) v = nl.
 Proof.
   intros; apply eq_sym.
+  replace (updN ol (wordToNat i) v) with (upd ol i v) by auto.
   eapply list2mem_array_upd; eauto.
 Qed.
 
-Theorem list2mem_array_removelast_eq : forall V (nl ol : list V),
-  (arrayN_ex ol (length ol - 1))%pred (list2mem nl)
+Theorem list2mem_array_removelast_eq : forall V (nl ol : list V) (b : addr),
+  (array_ex ol $ (length ol - 1))%pred (list2mem nl)
+  -> length ol <= wordToNat b
+  -> length nl <= wordToNat b
   -> length ol > 0
   -> nl = removelast ol.
 Proof.
-  unfold arrayN_ex; intros.
+  unfold array_ex; intros.
   destruct ol.
-  inversion H0.
+  inversion H2.
 
   eapply list2mem_array_eq with (l' := nl); eauto.
   pred_apply.
+  erewrite wordToNat_natToWord_bound with (bound:=b) by omega.
   rewrite firstn_removelast_eq; auto.
   rewrite skipn_oob by omega.
-  unfold arrayN at 2.
+  unfold array at 2.
   clear H; cancel.
+  rewrite length_removelast.
+  omega.
+  contradict H2; rewrite H2.
+  unfold length; omega.
 Qed.
 
 
 Theorem list2mem_array_exis : forall V l (def : V) i,
-  (arrayN_ex l i * i |-> selN l i def)%pred (list2mem l)
-  -> (arrayN_ex l i * i |->?)%pred (list2mem l).
+  (array_ex l i * i |-> sel l i def)%pred (list2mem l)
+  -> (array_ex l i * i |->?)%pred (list2mem l).
 Proof.
   intros; pred_apply; cancel.
 Qed.
@@ -463,7 +526,7 @@ Ltac rewrite_list2mem_pred :=
     first [
       is_var v; rewrite_list2mem_pred_sel H; subst v |
       match prd with
-      | arrayN_ex ?ol ix =>
+      | array_ex ?ol ix =>
         is_var l; rewrite_list2mem_pred_upd H;
         [ subst l | clear H .. ]
       end ]
@@ -473,9 +536,9 @@ Ltac list2mem_ptsto_cancel :=
   match goal with
   | [ |- (_ * ?p |-> ?a)%pred (list2mem ?l) ] =>
     let Hx := fresh in
-    assert (arrayN 0 l (list2mem l)) as Hx;
+    assert (array $0 l $1 (list2mem l)) as Hx;
       [ eapply list2mem_array; eauto; try omega |
-        pred_apply; erewrite arrayN_except; clear Hx;
+        pred_apply; erewrite array_except; unfold sel; clear Hx;
         try autorewrite with defaults; eauto ]
   end.
 
